<div class="cabecalho">

Transformação $\Delta - Y | Y - \Delta$

</div>
<div class="conteudo normal">

Aplicando os mesmos princípios para todos os terminais:

$$
\begin{align}
R_{xy} &= {{{1} \over {{{1} \over {R_{c}}} + {{1} \over {R_{a} + R_{b}}}}}} = {{R_{c} (R_{a} + R_{b})} \over {R_{a} + R_{b} + R_{c}}} = R_{1} + R_{2} \\
R_{xz} &= {{{1} \over {{{1} \over {R_{b}}} + {{1} \over {R_{a} + R_{c}}}}}} = {{R_{b} (R_{a} + R_{c})} \over {R_{a} + R_{b} + R_{c}}} = R_{1} + R_{3} \\
R_{yz} &= {{{1} \over {{{1} \over {R_{a}}} + {{1} \over {R_{b} + R_{c}}}}}} = {{R_{a} (R_{b} + R_{c})} \over {R_{a} + R_{b} + R_{c}}} = R_{2} + R_{3}
\end{align}
$$

</div>
